Make [resume_thread] and [suspend_thread] common for all concurrent machines. i.e. defined in concurrent_machine.v. this requires lifting the definitions of getThreadC and updThreadC. At this point, some proofs in compcert_threads.v should break, but it will be easily fixable.

compcomp/juicy_machine.v
@@ -72,10 +72,10 @@ Module ThreadPool.
   Section ThreadPool.
     
     Variable cT : Type.
-
+    Notation ctl':= (@ctl cT).
     Record t := mk
                   { num_threads : pos
-                    ; pool :> 'I_num_threads -> cT
+                    ; pool :> 'I_num_threads -> ctl'
                     ; juice : 'I_num_threads -> rmap;
                     lpool : LockPool
                                                 
@@ -96,7 +96,7 @@ End ThreadPool.
 Section poolDefs.
 
   Variable cT : Type.
-
+  Notation ctl':= (@ctl cT).
   Variable (tp : ThreadPool.t cT).
 
   Import ThreadPool.
@@ -145,7 +145,7 @@ Section poolDefs.
     @mk cT new_num_threads
         (fun (n : 'I_new_num_threads) => 
            match unlift new_tid n with
-             | None => c
+             | None => Kresume c
              | Some n' => tp n'
            end)
         (fun (n : 'I_new_num_threads) => 
@@ -199,11 +199,21 @@ Section poolDefs.
         discriminate.
   Defined.
   
-  Definition updThreadC (tid : 'I_num_threads) (c' : cT) : thread_pool :=
+  Definition updThreadC' (tid : 'I_num_threads) (c' : cT) : thread_pool :=
     @mk cT num_threads (fun (n : 'I_num_threads) =>
-                          if n == tid then c' else tp n) (juice tp)
+                          if n == tid then Krun c' else tp n) (juice tp)
         (lpool tp).
-
+  Definition containsThread: ThreadPool.t cT -> nat -> Prop:=
+    fun ms tid0 => tid0 < (ThreadPool.num_threads ms).
+  
+  Definition cont2ord {ms tid0} (cnt: containsThread ms tid0) :=
+    Ordinal cnt.
+  Set Printing All.
+  Definition updThreadC { tid0}(cnt: containsThread tp tid0) (c' : ctl) : tpool cT :=
+    @mk cT num_threads
+        (fun n => if n == (cont2ord cnt) then c' else (pool tp)  n)
+        (juice tp)
+        (lpool tp).
   Definition updThreadP (tid : 'I_num_threads) (pmap' : rmap) : thread_pool :=
     @mk cT num_threads (pool tp) (fun (n : 'I_num_threads) =>
                                     if n == tid then pmap' else (juice tp) n)
@@ -213,7 +223,7 @@ Section poolDefs.
     forall tid0 (Htid0 : tid0 < num_threads) (Hneq: tid <> tid0),
       joins ((juice tp) (Ordinal Htid0)) pmap.
   
-  Definition updThread (tid : 'I_num_threads) (c' : cT)
+  Definition updThread (tid : 'I_num_threads) (c' : ctl)
              (pmap : rmap): thread_pool :=
     @mk cT num_threads
         (fun (tid' : 'I_num_threads) =>
@@ -242,8 +252,12 @@ Section poolDefs.
       eapply Hwf. simpl; auto.
     - simpl in *. eapply Hrace_free; eauto.
   Defined.
+
   
-  Definition getThreadC (tid : 'I_num_threads) : cT := tp tid.
+  
+
+  Definition getThreadC {tid0 ms} (cnt: containsThread ms tid0) : ctl :=
+    (pool ms) (cont2ord cnt).
   
   Definition getThreadPerm (tid : 'I_num_threads) : rmap := (juice tp) tid.
 
@@ -273,9 +287,10 @@ Section poolLemmas.
   Context {cT : Type} (tp : ThreadPool.t cT).
 
   Import ThreadPool.
-
-  Lemma gssThreadCode (tid : 'I_(num_threads tp)) c' p' : 
-    getThreadC (updThread tp tid c' p') tid = c'.
+(*
+  Lemma gssThreadCode tid c' p' :
+    forall (cnt : containsThread (updThread tp (cont2ord cnt) c' p') tid),
+    getThreadC  ctn = c'.
   Proof. by rewrite /getThreadC /updThread /= eq_refl. Defined.
 
   Lemma gsoThread (tid tid' : 'I_(num_threads tp)) c' p':
@@ -294,6 +309,7 @@ Section poolLemmas.
     tid = ordinal_pos_incr (num_threads tp) ->
     getThreadC (addThread tp c pmap) tid = c.
   Proof. by rewrite /getThreadC /addThread /= => <-; rewrite unlift_none. Qed.
+*)
 (*
   Lemma permMapsInv_lt : forall m (Hinv: mem_compatible tp m) tid,
                            permMapLt (getThreadPerm tp tid) p.
@@ -445,10 +461,10 @@ Module Concur.
     Context {cT G : Type} {the_sem : CoreSemantics G cT mem}{LP:LockPool}.
     
     Notation cT' := (@ctl cT).
-    Notation thread_pool := (t cT').
+    Notation thread_pool := (t cT).
     Notation perm_map := rmap.
 
-    Definition containsThread: ThreadPool.t cT' -> nat -> Prop:=
+    Definition containsThread: ThreadPool.t cT -> nat -> Prop:=
       fun ms tid0 => tid0 < (ThreadPool.num_threads ms).
 
     Variable the_ge : G.
@@ -457,13 +473,12 @@ Module Concur.
     Record invariant tp :=
       { (*canonical : forall tid, isCanonical (juice tp tid);*)
         no_race : race_free tp;
-        lock_pool : forall (pf : 0 < num_threads tp), exists c,
-                      getThreadC tp (Ordinal pf) = Krun c /\ halted the_sem c
+        lock_pool : forall (cnt : containsThread tp 0), exists c,
+                      getThreadC cnt  = Krun c /\ halted the_sem c
       }.
     
     (* Semantics of the coarse-grained concurrent machine*)
-    Definition cont2ord {ms tid0} (cnt: containsThread ms tid0) :=
-      Ordinal cnt.
+    
 
     Definition personal_mem {tid0 tp m} (cnt: containsThread tp tid0)
                (Hcompatible: mem_compatible tp m): juicy_mem.
@@ -484,9 +499,9 @@ Module Concur.
           forall (Hpersonal_perm:
                personal_mem cnt Hcompatible = jm)
             (Hinv : invariant tp)
-            (Hthread: getThreadC tp tid = Krun c)
+            (Hthread: getThreadC cnt = Krun c)
             (Hcorestep: corestep juicy_sem the_ge c jm c' jm')
-            (Htp': tp' = @updThread cT' tp tid (Krun c') (m_phi jm'))
+            (Htp': tp' = @updThread cT tp tid (Krun c') (m_phi jm'))
             (Hm': m_dry jm' = m' ),
             juicy_step cnt Hcompatible tp' m'.
 
@@ -503,7 +518,7 @@ Module Concur.
           let: m' := m_dry jm' in
           forall
             (Hinv : invariant tp)
-            (Hthread: getThreadC tp tid = Kstop c)
+            (Hthread: getThreadC cnt0 = Kstop c)
             (Hat_external: at_external the_sem c =
                            Some (LOCK, ef_sig LOCK, Vptr b ofs::nil))
             (Hcompatible: mem_compatible tp m)
@@ -526,7 +541,7 @@ Module Concur.
           let: m' := m_dry jm' in
           forall
             (Hinv : invariant tp)
-            (Hthread: getThreadC tp tid = Kstop c)
+            (Hthread: getThreadC cnt0 = Kstop c)
             (Hat_external: at_external the_sem c =
                            Some (UNLOCK, ef_sig UNLOCK, Vptr b ofs::nil))
             (Hcompatible: mem_compatible tp m)
@@ -549,7 +564,7 @@ Module Concur.
           let: tid := cont2ord cnt0 in
           forall
             (Hinv : invariant tp)
-            (Hthread: getThreadC tp tid = Kstop c)
+            (Hthread: getThreadC cnt0 = Kstop c)
             (Hat_external: at_external the_sem c =
                            Some (CREATE, ef_sig CREATE, vf::arg::nil))
             (Hinitial: initial_core the_sem the_ge vf (arg::nil) = Some c_new)
@@ -563,7 +578,7 @@ Module Concur.
             (Hsat_fun_spec: P d_phi)
             (Hrem_fun_res: join d_phi phi' (m_phi jm))
             (Htp': tp_upd = updThread tp tid (Kresume c') phi')
-            (Htp': tp' = addThread tp_upd (Kresume c_new) d_phi),
+            (Htp': tp' = addThread tp_upd c_new d_phi),
             conc_step cnt0 Hcompat tp' m
                      
     | step_mklock :
@@ -574,7 +589,7 @@ Module Concur.
           let: m' := m_dry jm' in
           forall
             (Hinv : invariant tp)
-            (Hthread: getThreadC tp tid = Kstop c)
+            (Hthread: getThreadC cnt0 = Kstop c)
             (Hat_external: at_external the_sem c =
                            Some (MKLOCK, ef_sig MKLOCK, Vptr b ofs::nil))
             (Hcompatible: mem_compatible tp m)
@@ -605,7 +620,7 @@ Module Concur.
           let: m' := m_dry jm' in
           forall
             (Hinv : invariant tp)
-            (Hthread: getThreadC tp tid = Kstop c)
+            (Hthread: getThreadC cnt0 = Kstop c)
             (Hat_external: at_external the_sem c =
                            Some (FREE_LOCK, ef_sig FREE_LOCK, Vptr b ofs::nil))
             (Hcompatible: mem_compatible tp m)
@@ -634,7 +649,7 @@ Module Concur.
           let: phi := m_phi jm in
           forall
             (Hinv : invariant tp)
-            (Hthread: getThreadC tp tid = Kstop c)
+            (Hthread: getThreadC cnt0 = Kstop c)
             (Hat_external: at_external the_sem c =
                            Some (LOCK, ef_sig LOCK, Vptr b ofs::nil))
             (Hcompatible: mem_compatible tp m)
@@ -669,18 +684,17 @@ Module Concur.
     
     (*thread pool*)
     Import ThreadPool.  
-    Notation thread_pool := (t cT').  
+    Notation thread_pool := (t cT).  
     
     (*MACHINE VARIABLES*)
     Definition machine_state: Type:= thread_pool.
-    Definition containsThread: machine_state -> tid -> Prop:=
-      fun ms tid0 => tid0 < (num_threads ms).
-    Definition lp_id : tid:= (0)%nat.                            (* Useless *)
+    Definition containsThread: machine_state -> tid -> Prop:= containsThread.
+    Definition lp_id : tid:= (0)%nat. (*lock pool thread id*)
     
     (*INVARIANTS*)
     (*The state respects the memory*)
     Definition mem_compatible: machine_state -> mem -> Prop:=
-      @mem_compatible cT'.
+      @mem_compatible cT.
     
     (*Steps*)
     Definition cstep (genv:G): forall {tid0 ms m},
@@ -688,27 +702,6 @@ Module Concur.
                                  machine_state -> mem -> Prop:=
       @juicy_step cT G Sem genv.
     
-    Inductive resume_thread': forall {tid0} {ms:machine_state},
-                                containsThread ms tid0 -> machine_state -> Prop:=
-    | ResumeThread: forall tid0 ms ms' c
-                      (ctn: containsThread ms tid0)
-                      (HC: getThreadC ms (cont2ord ctn) = Kresume c)
-                      (Hms': updThreadC ms (cont2ord ctn) (Krun c)  = ms'),
-                      resume_thread' ctn ms'.
-    Definition resume_thread: forall {tid0 ms},
-                                containsThread ms tid0 -> machine_state -> Prop:=
-      @resume_thread'.
-
-    Inductive suspend_thread': forall {tid0} {ms:machine_state},
-                                 containsThread ms tid0 -> machine_state -> Prop:=
-    | SuspendThread: forall tid0 ms ms' c
-                       (ctn: containsThread ms tid0)
-                       (HC: getThreadC ms (cont2ord ctn) = Krun c)
-                       (Hms': updThreadC ms (cont2ord ctn) (Kstop c)  = ms'),
-                       suspend_thread' ctn ms'.
-    Definition suspend_thread : forall {tid0 ms},
-                                  containsThread ms tid0 -> machine_state -> Prop:=
-      @suspend_thread'.
     
     Definition conc_call (genv:G):
       forall {tid0 ms m}, (nat -> delta_map) -> containsThread ms tid0 -> mem_compatible ms m ->
@@ -719,12 +712,12 @@ Module Concur.
                                containsThread ms tid0 -> Prop:=
     | thread_halted':
         forall tp c tid0
-          (ctn: containsThread tp tid0),
-          let: tid := cont2ord ctn in
+          (cnt: containsThread tp tid0),
+          let: tid := cont2ord cnt in
           forall
-            (Hthread: getThreadC tp tid = Krun c)
+            (Hthread: getThreadC cnt = Krun c)
             (Hcant: halted Sem c),
-            threadHalted' ctn. 
+            threadHalted' cnt. 
     Definition threadHalted: forall {tid0 ms},
                                containsThread ms tid0 -> Prop:= @threadHalted'.
 
